proofs/toEC/refresh_for.v
@@ -1,5 +1,14 @@
 From mathcomp Require Import ssrbool eqtype.
-Require Import expr.
+Require Import compiler_util expr.
+
+Module Import E.
+
+  Definition pass : string := "refresh for".
+
+  Definition fresh_error (ii : instr_info) :=
+    pp_internal_error_s_at pass ii "fresh for-counter is not fresh".
+
+End E.
 
 Section REFRESH_FOR.
 
@@ -10,56 +19,72 @@ Context
   (always : bool)
 .
 
+#[local] Existing Instance progUnit.
+
 Definition refresh_for_clone (ii : instr_info) (x : var) : var :=
   let n := x.(vname) in
   let n' := fresh_var_ident (Ident.id_kind n) ii (Ident.id_name n) x.(vtype) in
   {| vtype := x.(vtype); vname := n'; |}.
 
-Let refresh_for_ii_aux rf (i : instr) : instr :=
-  let 'MkI ii ir := i in MkI ii (rf ii ir).
+Let refresh_for_ii_aux rf (i : instr) : cexec instr :=
+  let 'MkI ii ir := i in
+  Let ir' := rf ii ir in
+  ok (MkI ii ir').
 
-Let refresh_for_c_aux rf (c : cmd) : cmd := map (refresh_for_ii_aux rf) c.
+Let refresh_for_c_aux rf (c : cmd) : cexec cmd :=
+  mapM (refresh_for_ii_aux rf) c.
 
-Fixpoint refresh_for_i (ii : instr_info) (i : instr_r) : instr_r :=
-  let rec := refresh_for_c_aux refresh_for_i in
+Fixpoint refresh_for_i
+  (V : Sv.t) (ii : instr_info) (i : instr_r) : cexec instr_r :=
+  let rec := refresh_for_c_aux (refresh_for_i V) in
   match i with
   | Cassgn _ _ _ _ | Copn _ _ _ _ | Csyscall _ _ _ | Cassert _ | Ccall _ _ _ =>
-    i
-  | Cif e c1 c2 => Cif e (rec c1) (rec c2)
-  | Cwhile al c1 e info c2 => Cwhile al (rec c1) e info (rec c2)
+    ok i
+  | Cif e c1 c2 =>
+    Let c1 := rec c1 in
+    Let c2 := rec c2 in
+    ok (Cif e c1 c2)
+  | Cwhile al c1 e info c2 =>
+    Let c1 := rec c1 in
+    Let c2 := rec c2 in
+    ok (Cwhile al c1 e info c2)
   | Cfor x r c =>
       if always || Sv.mem x (write_c c) then
         let x' := refresh_for_clone ii x.(v_var) in
+        Let _ := assert (~~ Sv.mem x' V) (E.fresh_error ii) in
         let xi' := {| v_var := x'; v_info := x.(v_info); |} in
         let cpy :=
           MkI ii (Cassgn (Lvar x) AT_inline x.(v_var).(vtype) (Plvar xi'))
         in
-        Cfor xi' r (cpy :: rec c)
-      else Cfor x r (rec c)
+        Let c := rec c in
+        ok (Cfor xi' r (cpy :: c))
+      else
+        Let c := rec c in
+        ok (Cfor x r c)
   end.
 
-Definition refresh_for_ii := refresh_for_ii_aux refresh_for_i.
-Definition refresh_for_c := refresh_for_c_aux refresh_for_i.
+Definition refresh_for_ii (V : Sv.t) := refresh_for_ii_aux (refresh_for_i V).
+Definition refresh_for_c (V : Sv.t) := refresh_for_c_aux (refresh_for_i V).
 
-Definition refresh_for_fd (fd : _fundef unit) : _fundef unit :=
-  {|
+Definition refresh_for_fd
+  (V : Sv.t) (fd : _fundef unit) : cexec (_fundef unit) :=
+  Let c := refresh_for_c V fd.(f_body) in
+  ok {|
     f_info := f_info fd;
     f_contract := f_contract fd;
     f_tyin := f_tyin fd;
     f_params := f_params fd;
-    f_body := refresh_for_c fd.(f_body);
+    f_body := c;
     f_tyout := f_tyout fd;
     f_res := f_res fd;
     f_extra := f_extra fd;
   |}.
 
-Definition refresh_for_fun_decl
-  (fd : funname * _fundef unit) : funname * _fundef unit :=
-  let '(fn, fd) := fd in (fn, refresh_for_fd fd).
-
-Definition refresh_for_prog (p : _uprog) : _uprog :=
-  {|
-    p_funcs := map refresh_for_fun_decl (p_funcs p);
+Definition refresh_for_prog (p : _uprog) : cexec _uprog :=
+  let V := vars_p (p_funcs p) in
+  Let funcs := map_cfprog (refresh_for_fd V) (p_funcs p) in
+  ok {|
+    p_funcs := funcs;
     p_globs := p_globs p;
     p_extra := p_extra p;
   |}.
