proofs/toEC/toEC_jazz.v
@@ -1,6 +1,8 @@
-Require Import expr.
+Require Import compiler_util expr.
 Require Import normalize_cond.
 Require Import refresh_for.
+Require Import for_to_while.
+Require Import flatten_while.
 
 Section TOEC.
 
@@ -10,7 +12,9 @@ Context
   (fresh_var_ident : v_kind -> instr_info -> string -> atype -> Ident.ident)
 .
 
-Definition toEC_prog (p : _uprog) : _uprog :=
-  refresh_for_prog fresh_var_ident false (normalize_cond_prog p).
+Definition toEC_prog (normal : bool) (p : _uprog) : cexec _uprog :=
+  Let p1 := refresh_for_prog fresh_var_ident false (normalize_cond_prog p) in
+  Let p2 := if normal then for_to_while_prog fresh_var_ident p1 else ok p1 in
+  ok (flatten_while_prog p2).
 
 End TOEC.
