proofs/toEC/flatten_while_proof.v
@@ -1,0 +1,34 @@
+From mathcomp Require Import ssreflect ssrfun ssrbool eqtype.
+
+Require Import psem.
+Require Export flatten_while.
+
+Section FLATTEN_WHILE_PROOF.
+
+Context
+  {wsw : WithSubWord}
+  {dc : DirectCall}
+  {asm_op syscall_state : Type}
+  {ep : EstateParams syscall_state}
+  {spp : SemPexprParams}
+  {sip : SemInstrParams asm_op syscall_state}
+  {E E0 : Type -> Type}
+  {wE : with_Error E E0}
+  {rE0 : EventRels E0}
+.
+
+#[local] Existing Instance progUnit.
+#[local] Existing Instance sCP_unit.
+
+Context
+  (p p' : uprog)
+  (ev : extra_val_t)
+  (flatten_while_ok : flatten_while_prog p = p')
+.
+
+Lemma flatten_while_proof fn :
+  wiequiv_f p p' ev ev (rpreF (eS := eq_spec)) fn fn (rpostF (eS := eq_spec)).
+Proof using flatten_while_ok.
+Admitted.
+
+End FLATTEN_WHILE_PROOF.
