proofs/toEC/refresh_for_proof.v
@@ -1,6 +1,6 @@
 From mathcomp Require Import ssreflect ssrfun ssrbool eqtype.
 
-Require Import psem.
+Require Import psem compiler_util.
 Require Export refresh_for.
 
 Section REFRESH_FOR_PROOF.
@@ -25,16 +25,20 @@ Context
   (always : bool)
   (p p' : uprog)
   (ev : extra_val_t)
-  (refresh_for_ok : refresh_for_prog fresh_var_ident always p = p')
-  (fresh_var_ident_fresh :
-     forall (ii : instr_info) (x : var),
-       ~ Sv.In (refresh_for_clone fresh_var_ident ii x) (vars_p (p_funcs p)))
+  (refresh_for_ok : refresh_for_prog fresh_var_ident always p = ok p')
 .
 
 Let X := vars_p (p_funcs p).
 
 Lemma refresh_for_eq_globs : p_globs p = p_globs p'.
-Proof using refresh_for_ok. by rewrite -refresh_for_ok. Qed.
+Proof using refresh_for_ok.
+  by move: refresh_for_ok; rewrite /refresh_for_prog; t_xrbindP => ?? <-.
+Qed.
+
+Lemma refresh_for_eq_extra : p_extra p = p_extra p'.
+Proof using refresh_for_ok.
+  by move: refresh_for_ok; rewrite /refresh_for_prog; t_xrbindP => ?? <-.
+Qed.
 
 #[local] Instance refresh_for_checker_st_eq_onP :
   Checker_eq p p' checker_st_eq_on :=
@@ -45,74 +49,90 @@ Proof using refresh_for_ok. by rewrite -refresh_for_ok. Qed.
   checker_a_st_eq_onP refresh_for_eq_globs.
 
 Let Pi (i : instr) :=
+  forall i',
+  refresh_for_ii fresh_var_ident always X i = ok i' ->
   Sv.Subset (read_I i) X ->
-  wequiv_rec p p' ev ev eq_spec (st_eq_on X)
-    [:: i] [:: refresh_for_ii fresh_var_ident always i] (st_eq_on X).
+  wequiv_rec p p' ev ev eq_spec (st_eq_on X) [:: i] [:: i'] (st_eq_on X).
 
 Let Pi_r (i : instr_r) :=
-  forall ii, Sv.Subset (read_i i) X ->
+  forall ii i',
+  refresh_for_i fresh_var_ident always X ii i = ok i' ->
+  Sv.Subset (read_i i) X ->
   wequiv_rec p p' ev ev eq_spec (st_eq_on X)
-    [:: MkI ii i]
-    [:: refresh_for_ii fresh_var_ident always (MkI ii i)]
-    (st_eq_on X).
+    [:: MkI ii i] [:: MkI ii i'] (st_eq_on X).
 
 Let Pc (c : cmd) :=
+  forall c',
+  refresh_for_c fresh_var_ident always X c = ok c' ->
   Sv.Subset (read_c c) X ->
-  wequiv_rec p p' ev ev eq_spec (st_eq_on X)
-    c (refresh_for_c fresh_var_ident always c) (st_eq_on X).
+  wequiv_rec p p' ev ev eq_spec (st_eq_on X) c c' (st_eq_on X).
 
 Lemma refresh_for_cP c : Pc c.
-Proof using fresh_var_ident_fresh refresh_for_ok.
+Proof using refresh_for_ok.
 apply: (cmd_rect (Pr := Pi_r) (Pi := Pi) (Pc := Pc)) => // {c}.
-+ by move=> i ii hi hsub; apply hi.
-+ by move=> hsub; apply wequiv_nil.
-+ move=> i c hi hc hsub; move: hsub; rewrite read_c_cons => hsub.
++ move=> i ii hi i' heq hsub.
+  move: heq; rewrite /refresh_for_ii /=.
+  t_xrbindP => ir' hir' <-.
+  exact: (hi ii ir' hir' hsub).
++ move=> c' heq hsub.
+  move: heq; rewrite /refresh_for_c /= => -[<-].
+  by apply wequiv_nil.
++ move=> i c hi hc c' heq hsub; move: hsub; rewrite read_c_cons => hsub.
+  move: heq; rewrite /refresh_for_c /=.
+  t_xrbindP => i2 hi2 c2 hc2 <-.
   apply wequiv_cons with (st_eq_on X).
-  - by apply hi; SvD.fsetdec.
-  by apply hc; SvD.fsetdec.
-+ move=> x tg ty e ii hsub; move: hsub; rewrite read_i_assgn => hsub.
+  - apply: (hi _ hi2); SvD.fsetdec.
+  apply: (hc _ hc2); SvD.fsetdec.
++ move=> x tg ty e ii i' heq hsub.
+  move: heq => /ok_inj <-.
+  move: hsub; rewrite read_i_assgn => hsub.
   apply wequiv_assgn_rel_eq with checker_st_eq_on X => //=.
   - exact: refresh_for_checker_st_eq_onP.
   - by split=>//; rewrite /read_es /= read_eE; SvD.fsetdec.
-  - split=>//.
-    + by SvD.fsetdec.
-    by rewrite /read_rvs /= read_rvE; SvD.fsetdec.
-+ move=> xs t o es ii hsub; move: hsub; rewrite read_i_opn => hsub.
+  split=>//.
+  + by SvD.fsetdec.
+  by rewrite /read_rvs /= read_rvE; SvD.fsetdec.
++ move=> xs t o es ii i' heq hsub.
+  move: heq => /ok_inj <-.
+  move: hsub; rewrite read_i_opn => hsub.
   apply wequiv_opn_rel_eq with checker_st_eq_on X => //=.
   - exact: refresh_for_checker_st_eq_onP.
   - by split=>//; SvD.fsetdec.
   by split=>//; SvD.fsetdec.
-+ move=> xs o es ii hsub; move: hsub; rewrite read_i_syscall => hsub.
++ move=> xs o es ii i' heq hsub.
+  move: heq => /ok_inj <-.
+  move: hsub; rewrite read_i_syscall => hsub.
   apply wequiv_syscall_rel_eq_core with checker_st_eq_on X => //.
   - exact: refresh_for_checker_st_eq_onP.
   - by split=>//; SvD.fsetdec.
   - by split=>//; SvD.fsetdec.
   by move=> > <- ->; eauto.
-+ move=> a ii hsub; move: hsub; rewrite read_i_assert => hsub.
++ move=> a ii i' heq hsub.
+  move: heq => /ok_inj <-.
+  move: hsub; rewrite read_i_assert => hsub.
   apply wequiv_assert_rel_eq with checker_a_st_eq_on => //.
   - exact: refresh_for_checker_a_st_eq_onP.
   by split=>//.
-+ move=> e c1 c2 hc1 hc2 ii hsub; move: hsub; rewrite read_i_if => hsub.
++ move=> e c1 c2 hc1 hc2 ii i' heq hsub; move: hsub; rewrite read_i_if => hsub.
+  move: heq; rewrite /=; t_xrbindP => c1' hc1' c2' hc2' <-.
   apply wequiv_if_rel_eq with checker_st_eq_on X X X => //.
   - exact: refresh_for_checker_st_eq_onP.
   - by split=>//; rewrite /read_es /= read_eE; SvD.fsetdec.
-  - by apply hc1; SvD.fsetdec.
-  by apply hc2; SvD.fsetdec.
-+ move=> v dir lo hi c hc ii hsub.
-  rewrite /Pi_r.
-  rewrite /refresh_for_ii /=.
+  - apply: (hc1 _ hc1'); SvD.fsetdec.
+  apply: (hc2 _ hc2'); SvD.fsetdec.
++ move=> v dir lo hi c hc ii i' heq hsub.
+  move: hsub; rewrite read_i_for => hsub.
+  move: heq; rewrite /=.
   case: ifP => htrig; last first.
-  - apply wequiv_for_rel_eq with checker_st_eq_on X X => //.
+  - t_xrbindP => c2 hc2 <-.
+    apply wequiv_for_rel_eq with checker_st_eq_on X X => //.
     + exact: refresh_for_checker_st_eq_onP.
-    + by split=>//; rewrite /read_es /= !read_eE;
-        move: hsub; rewrite read_i_for; SvD.fsetdec.
-    + by split=>//; move: hsub; rewrite read_i_for; SvD.fsetdec.
-    by apply hc; move: hsub; rewrite read_i_for; SvD.fsetdec.
-  have hfresh : ~ Sv.In (refresh_for_clone fresh_var_ident ii (v_var v)) X
-    by apply: fresh_var_ident_fresh.
+    + by split=>//; rewrite /read_es /= !read_eE; SvD.fsetdec.
+    + by split=>//; SvD.fsetdec.
+    apply: (hc _ hc2); SvD.fsetdec.
   set x' := refresh_for_clone fresh_var_ident ii (v_var v).
+  t_xrbindP => /Sv_memP hfresh c2 hc2 <-.
   set xi' := {| v_var := x'; v_info := v_info v |}.
-  have hsub' := hsub; move: hsub'; rewrite read_i_for => hsub'.
   apply (wequiv_for (P0 := st_eq_on X) (P := st_eq_on X)
     (Pi := fun s1 s2 =>
       st_eq_on (Sv.remove v X) s1 s2 /\ (evm s2).[x'] = (evm s1).[v]
@@ -123,7 +143,7 @@ apply: (cmd_rect (Pr := Pi_r) (Pi := Pi) (Pc := Pc)) => // {c}.
     move=> s1 s2 vs hst hev.
     have [vs' hvs' heq] :=
       read_es_st_eq_on (X:=X) (wdb:=true) (gd:=p_globs p) (es:=[::lo;hi])
-        (ltac:(move: hsub'; rewrite /read_es /= !read_eE; SvD.fsetdec)) hst hev.
+        (ltac:(rewrite /read_es /= !read_eE; SvD.fsetdec)) hst hev.
     exists vs' => //.
     by rewrite heq; exact: values_uincl_refl.
   - move=> i s1 s2 s1out hst hw1.
@@ -141,13 +161,13 @@ apply: (cmd_rect (Pr := Pi_r) (Pi := Pi) (Pc := Pc)) => // {c}.
       move=> y hy; move: hy; rewrite Sv.remove_spec => -[hyX hyv].
       rewrite !Vm.setP_neq.
       + by case: hst => _ _ /(_ y hyX).
-      + by apply/eqP => heq; apply: hfresh; change (Sv.In x' X); rewrite heq.
-      by apply/eqP => heq; apply: hyv; rewrite heq.
+      + by apply/eqP => heqq; apply: hfresh; change (Sv.In x' X); rewrite heqq.
+      by apply/eqP => heqq; apply: hyv; rewrite heqq.
     - by rewrite !Vm.setP_eq.
     by exists i; rewrite Vm.setP_eq heqty.
   apply (wequiv_cat (R := st_eq_on X) (c1 := [::]) (c1' := c)
     (c2 := [:: MkI ii (Cassgn v AT_inline (vtype v) (Plvar xi'))])
-    (c2' := refresh_for_c fresh_var_ident always c)).
+    (c2' := c2)).
   - apply (wequiv_assign_right p ev ev
       (P := fun s1 s2 =>
         st_eq_on (Sv.remove v X) s1 s2 /\ (evm s2).[x'] = (evm s1).[v]
@@ -169,22 +189,26 @@ apply: (cmd_rect (Pr := Pi_r) (Pi := Pi) (Pc := Pc)) => // {c}.
     - by case: hst.
     - by case: hst.
     move=> y hy.
-    have [heq|hne] := eqVneq y (v_var v).
-    - by rewrite heq Vm.setP_eq heqty.
+    have [heqq|hne] := eqVneq y (v_var v).
+    - by rewrite heqq Vm.setP_eq heqty.
     have hne' : v_var v != y by rewrite eq_sym.
     rewrite (Vm.setP_neq _ (Vint z) hne').
     case: hst => _ _ /(_ y); apply.
     rewrite Sv.remove_spec; split=>//.
     by move/eqP: hne.
-  apply: hc.
-  by move: hsub'; clear; SvD.fsetdec.
-+ move=> a c e info c' hc hc' ii hsub; move: hsub; rewrite read_i_while => hsub.
+  apply: (hc _ hc2).
+  by clear -hsub; SvD.fsetdec.
++ move=> a c1 e info c2 hc1 hc2 ii i' heq hsub.
+  move: hsub; rewrite read_i_while => hsub.
+  move: heq; rewrite /=; t_xrbindP => c1' hc1' c2' hc2' <-.
   apply wequiv_while_rel_eq with checker_st_eq_on X => //.
   - exact: refresh_for_checker_st_eq_onP.
   - by split=>//; rewrite /read_es /= read_eE; SvD.fsetdec.
-  - by apply hc; SvD.fsetdec.
-  by apply hc'; SvD.fsetdec.
-move=> xs f es ii hsub; move: hsub; rewrite read_i_call => hsub.
+  - apply: (hc1 _ hc1'); SvD.fsetdec.
+  apply: (hc2 _ hc2'); SvD.fsetdec.
+move=> xs f es ii i' heq hsub.
+move: heq => /ok_inj <-.
+move: hsub; rewrite read_i_call => hsub.
 apply wequiv_call_rel_eq with checker_st_eq_on X => //.
 - exact: refresh_for_checker_st_eq_onP.
 - by split=>//; SvD.fsetdec.
@@ -192,28 +216,32 @@ apply wequiv_call_rel_eq with checker_st_eq_on X => //.
 move=> ?? <-; exact/wequiv_fun_rec.
 Qed.
 
-Lemma get_fundef_refresh_for fn :
-  get_fundef (p_funcs p') fn =
-    omap (refresh_for_fd fresh_var_ident always) (get_fundef (p_funcs p) fn).
+Lemma refresh_for_all_checked fn fd1 :
+  get_fundef (p_funcs p) fn = Some fd1 ->
+  exists2 fd2,
+    refresh_for_fd fresh_var_ident always X fd1 = ok fd2 &
+    get_fundef (p_funcs p') fn = Some fd2.
 Proof using refresh_for_ok.
-  rewrite -refresh_for_ok /refresh_for_prog /=.
-  by elim: (p_funcs p) => [|[fn' fd'] pfuns ih] //=; case: eqP.
+  move: refresh_for_ok; rewrite /refresh_for_prog; t_xrbindP => fds h1 <- hf.
+  apply: (get_map_cfprog_gen h1 hf).
 Qed.
 
 Lemma refresh_for_proof fn :
   wiequiv_f p p' ev ev (rpreF (eS := eq_spec)) fn fn (rpostF (eS := eq_spec)).
-Proof using refresh_for_ok fresh_var_ident_fresh.
+Proof using refresh_for_ok.
 apply wequiv_fun_ind => {}fn _ fs _ [<- <-] fd hget.
-exists (refresh_for_fd fresh_var_ident always fd).
-- by rewrite get_fundef_refresh_for hget.
+have [fd' hfd' hget'] := refresh_for_all_checked hget.
+exists fd'.
+- exact: hget'.
+move: hfd'; rewrite /refresh_for_fd; t_xrbindP => c hc <-.
 move=> s11 hinit.
 exists s11.
-- by apply: (eq_initialize _ _ _ _ hinit) => //; rewrite -refresh_for_ok.
+- by apply: (eq_initialize _ _ _ _ hinit) => //; rewrite -refresh_for_eq_extra.
 have hsubfd : Sv.Subset (vars_fd fd) X := vars_pP hget.
 have hsubc : Sv.Subset (read_c (f_body fd)) X.
   by move: hsubfd; rewrite /vars_fd /vars_c; SvD.fsetdec.
 exists (st_eq_on X), (st_eq_on X); split=> //.
-- exact: refresh_for_cP.
+- exact: (refresh_for_cP hc hsubc).
 apply: (wrequiv_weaken (P := st_eq_on (vars_l (f_res fd))) (Q := eq)) => //.
 - by move=> s t; apply: st_rel_weaken => vm1 vm2; apply: eq_onI;
     move: hsubfd; rewrite /vars_fd; SvD.fsetdec.
