proofs/toEC/toEC_jazz_proof.v
@@ -3,6 +3,8 @@ Require Import psem.
 Require Export toEC_jazz.
 Require Import normalize_cond_proof.
 Require Import refresh_for_proof.
+Require Import for_to_while_proof.
+Require Import flatten_while_proof.
 Import Utf8.
 
 Section TOEC_PROOF.
@@ -25,18 +27,16 @@ Context
 
 Context
   (fresh_var_ident : v_kind -> instr_info -> string -> atype -> Ident.ident)
+  (normal : bool)
   (p p' : uprog)
   (ev : extra_val_t)
-  (toEC_ok : toEC_prog fresh_var_ident p = p')
-  (fresh_var_ident_fresh :
-     forall (ii : instr_info) (x : var),
-       ~ Sv.In (refresh_for_clone fresh_var_ident ii x)
-         (vars_p (p_funcs (normalize_cond_prog p))))
+  (toEC_ok : toEC_prog fresh_var_ident normal p = ok p')
 .
 
 Lemma it_toEC_progP fn :
   wiequiv_f p p' ev ev (rpreF (eS := eq_spec)) fn fn (rpostF (eS := eq_spec)).
-Proof using toEC_ok rE0_trans fresh_var_ident_fresh.
+Proof using toEC_ok rE0_trans.
+move: toEC_ok; rewrite /toEC_prog; t_xrbindP => p1 hrefresh p2 hp2eq hflatten.
 have hp1 :=
   normalize_cond_proof
     (wsw:=wsw) (dc:=dc) (asm_op:=asm_op) (syscall_state:=syscall_state)
@@ -47,8 +47,33 @@ have hp2 :=
     (wsw:=wsw) (dc:=dc) (asm_op:=asm_op) (syscall_state:=syscall_state)
     (ep:=ep) (spp:=spp) (sip:=sip) (E:=E) (E0:=E0) (wE:=wE) (rE0:=rE0)
     (fresh_var_ident := fresh_var_ident) (always := false)
-    (p := normalize_cond_prog p) (fn := fn) ev toEC_ok fresh_var_ident_fresh.
-move: hp1 hp2; apply wiequiv_f_trans => //.
+    (p := normalize_cond_prog p) (fn := fn) ev hrefresh.
+have hp12 :
+  wiequiv_f p (to_uprog p1) ev ev
+    (rpreF (eS := eq_spec)) fn fn (rpostF (eS := eq_spec)).
+- move: hp1 hp2; apply wiequiv_f_trans => //.
+  + by move=> fs1 fs3 [_ <-]; exists fs1.
+  by move=> fs1 fs2 fs3 r1 r3 _ _ [r2 -> ->].
+have hp123 :
+  wiequiv_f p (to_uprog p2) ev ev
+    (rpreF (eS := eq_spec)) fn fn (rpostF (eS := eq_spec)).
+- move: hp2eq; case: normal => /=.
+  + move=> hp3.
+    have hp4 :=
+      for_to_while_proof
+        (wsw:=wsw) (dc:=dc) (asm_op:=asm_op) (syscall_state:=syscall_state)
+        (ep:=ep) (spp:=spp) (sip:=sip) (E:=E) (E0:=E0) (wE:=wE) (rE0:=rE0)
+        (fresh_var_ident := fresh_var_ident) (p := p1) (fn := fn) ev hp3.
+    move: hp12 hp4; apply wiequiv_f_trans => //.
+    * by move=> fs1 fs3 [_ <-]; exists fs1.
+    by move=> fs1 fs2 fs3 r1 r3 _ _ [r2 -> ->].
+  by move=> /ok_inj <-; exact hp12.
+have hp5 :=
+  flatten_while_proof
+    (wsw:=wsw) (dc:=dc) (asm_op:=asm_op) (syscall_state:=syscall_state)
+    (ep:=ep) (spp:=spp) (sip:=sip) (E:=E) (E0:=E0) (wE:=wE) (rE0:=rE0)
+    (p := p2) (fn := fn) ev hflatten.
+move: hp123 hp5; apply wiequiv_f_trans => //.
 - by move=> fs1 fs3 [_ <-]; exists fs1.
 by move=> fs1 fs2 fs3 r1 r3 _ _ [r2 -> ->].
 Qed.
